sequential composition; still long way to go..

arm/proofs/bignum_emontredc_8n_neon2.ml
@@ -38,7 +38,176 @@ let WORD_SUB2 = MESON [WORD_SUB] `y <= x ==> word_sub (word x) (word y):int64 = 
 let WORD_ADD_SUB = WORD_RULE
     `word_add (word_sub x (word y)) (word z):(N)word = word_add x (word_sub (word z) (word y))`;;
 
-let maddloop_step2_full_ops:int list = [
+
+(* The basic blocks 'outerloop' + 'maddloop' + 'loop_postamble'. *)
+let outerloop_step2_ops:int list = [
+  0xf94003e3;       (* arm_LDR X3 SP (Immediate_Offset (word 0)) *)
+  0xa9404c31;       (* arm_LDP X17 X19 X1 (Immediate_Offset (iword (&0))) *)
+  0xa9415434;       (* arm_LDP X20 X21 X1 (Immediate_Offset (iword (&16))) *)
+  0xa9402448;       (* arm_LDP X8 X9 X2 (Immediate_Offset (iword (&0))) *)
+  0xa9412c4a;       (* arm_LDP X10 X11 X2 (Immediate_Offset (iword (&16))) *)
+  0x3dc00455;       (* arm_LDR Q21 X2 (Immediate_Offset (word 16)) *)
+  0x9b037e24;       (* arm_MUL X4 X17 X3 *)
+  0x4e080c80;       (* arm_DUP_GEN Q0 X4 *)
+  0x4e955aa3;       (* arm_UZP2 Q3 Q21 Q21 32 *)
+  0x0ea12804;       (* arm_XTN Q4 Q0 32 *)
+  0x0ea12aa5;       (* arm_XTN Q5 Q21 32 *)
+  0x4ea00abc;       (* arm_REV64_VEC Q28 Q21 32 *)
+  0x2ea5c086;       (* arm_UMULL_VEC Q6 Q4 Q5 32 *)
+  0x2ea3c087;       (* arm_UMULL_VEC Q7 Q4 Q3 32 *)
+  0x4e805810;       (* arm_UZP2 Q16 Q0 Q0 32 *)
+  0x4ea09f80;       (* arm_MUL_VEC Q0 Q28 Q0 32 128 *)
+  0x6f6014c7;       (* arm_USRA_VEC Q7 Q6 32 64 128 *)
+  0x2ea3c201;       (* arm_UMULL_VEC Q1 Q16 Q3 32 *)
+  0x6ea02800;       (* arm_UADDLP Q0 Q0 32 *)
+  0x4e3d1ce2;       (* arm_AND_VEC Q2 Q7 Q29 128 *)
+  0x2ea58202;       (* arm_UMLAL_VEC Q2 Q16 Q5 32 *)
+  0x4f605400;       (* arm_SHL_VEC Q0 Q0 32 64 128 *)
+  0x6f6014e1;       (* arm_USRA_VEC Q1 Q7 32 64 128 *)
+  0x2ea58080;       (* arm_UMLAL_VEC Q0 Q4 Q5 32 *)
+  0x6f601441;       (* arm_USRA_VEC Q1 Q2 32 64 128 *)
+  0x4e083c0e;       (* arm_UMOV X14 Q0 0 8 *)
+  0x4e183c0f;       (* arm_UMOV X15 Q0 1 8 *)
+  0x9b087c8c;       (* arm_MUL X12 X4 X8 *)
+  0xab0c0231;       (* arm_ADDS X17 X17 X12 *)
+  0x9bc87c8c;       (* arm_UMULH X12 X4 X8 *)
+  0x9b097c8d;       (* arm_MUL X13 X4 X9 *)
+  0xba0d0273;       (* arm_ADCS X19 X19 X13 *)
+  0x9bc97c8d;       (* arm_UMULH X13 X4 X9 *)
+  0xba0e0294;       (* arm_ADCS X20 X20 X14 *)
+  0xba0f02b5;       (* arm_ADCS X21 X21 X15 *)
+  0x4e083c2e;       (* arm_UMOV X14 Q1 0 8 *)
+  0x4e183c2f;       (* arm_UMOV X15 Q1 1 8 *)
+  0x9a1f03f6;       (* arm_ADC X22 XZR XZR *)
+  0xab0c0273;       (* arm_ADDS X19 X19 X12 *)
+  0xba0d0294;       (* arm_ADCS X20 X20 X13 *)
+  0xba0e02b5;       (* arm_ADCS X21 X21 X14 *)
+  0x9a0f02d6;       (* arm_ADC X22 X22 X15 *)
+  0x9b037e65;       (* arm_MUL X5 X19 X3 *)
+  0x4e080ca0;       (* arm_DUP_GEN Q0 X5 *)
+  0x4e955aa3;       (* arm_UZP2 Q3 Q21 Q21 32 *)
+  0x0ea12804;       (* arm_XTN Q4 Q0 32 *)
+  0x0ea12aa5;       (* arm_XTN Q5 Q21 32 *)
+  0x4ea00abc;       (* arm_REV64_VEC Q28 Q21 32 *)
+  0x2ea5c086;       (* arm_UMULL_VEC Q6 Q4 Q5 32 *)
+  0x2ea3c087;       (* arm_UMULL_VEC Q7 Q4 Q3 32 *)
+  0x4e805810;       (* arm_UZP2 Q16 Q0 Q0 32 *)
+  0x4ea09f80;       (* arm_MUL_VEC Q0 Q28 Q0 32 128 *)
+  0x6f6014c7;       (* arm_USRA_VEC Q7 Q6 32 64 128 *)
+  0x2ea3c201;       (* arm_UMULL_VEC Q1 Q16 Q3 32 *)
+  0x6ea02800;       (* arm_UADDLP Q0 Q0 32 *)
+  0x4e3d1ce2;       (* arm_AND_VEC Q2 Q7 Q29 128 *)
+  0x2ea58202;       (* arm_UMLAL_VEC Q2 Q16 Q5 32 *)
+  0x4f605400;       (* arm_SHL_VEC Q0 Q0 32 64 128 *)
+  0x6f6014e1;       (* arm_USRA_VEC Q1 Q7 32 64 128 *)
+  0x2ea58080;       (* arm_UMLAL_VEC Q0 Q4 Q5 32 *)
+  0x6f601441;       (* arm_USRA_VEC Q1 Q2 32 64 128 *)
+  0x4e083c0e;       (* arm_UMOV X14 Q0 0 8 *)
+  0x4e183c0f;       (* arm_UMOV X15 Q0 1 8 *)
+  0x9b087cac;       (* arm_MUL X12 X5 X8 *)
+  0xab0c0273;       (* arm_ADDS X19 X19 X12 *)
+  0x9bc87cac;       (* arm_UMULH X12 X5 X8 *)
+  0x9b097cad;       (* arm_MUL X13 X5 X9 *)
+  0xba0d0294;       (* arm_ADCS X20 X20 X13 *)
+  0x9bc97cad;       (* arm_UMULH X13 X5 X9 *)
+  0xba0e02b5;       (* arm_ADCS X21 X21 X14 *)
+  0xba0f02d6;       (* arm_ADCS X22 X22 X15 *)
+  0x4e083c2e;       (* arm_UMOV X14 Q1 0 8 *)
+  0x4e183c2f;       (* arm_UMOV X15 Q1 1 8 *)
+  0x9a1f03f7;       (* arm_ADC X23 XZR XZR *)
+  0xab0c0294;       (* arm_ADDS X20 X20 X12 *)
+  0xba0d02b5;       (* arm_ADCS X21 X21 X13 *)
+  0xba0e02d6;       (* arm_ADCS X22 X22 X14 *)
+  0x9a0f02f7;       (* arm_ADC X23 X23 X15 *)
+  0xa9001424;       (* arm_STP X4 X5 X1 (Immediate_Offset (iword (&0))) *)
+  0x9b037e86;       (* arm_MUL X6 X20 X3 *)
+  0x4e080cc0;       (* arm_DUP_GEN Q0 X6 *)
+  0x4e955aa3;       (* arm_UZP2 Q3 Q21 Q21 32 *)
+  0x0ea12804;       (* arm_XTN Q4 Q0 32 *)
+  0x0ea12aa5;       (* arm_XTN Q5 Q21 32 *)
+  0x4ea00abc;       (* arm_REV64_VEC Q28 Q21 32 *)
+  0x2ea5c086;       (* arm_UMULL_VEC Q6 Q4 Q5 32 *)
+  0x2ea3c087;       (* arm_UMULL_VEC Q7 Q4 Q3 32 *)
+  0x4e805810;       (* arm_UZP2 Q16 Q0 Q0 32 *)
+  0x4ea09f80;       (* arm_MUL_VEC Q0 Q28 Q0 32 128 *)
+  0x6f6014c7;       (* arm_USRA_VEC Q7 Q6 32 64 128 *)
+  0x2ea3c201;       (* arm_UMULL_VEC Q1 Q16 Q3 32 *)
+  0x6ea02800;       (* arm_UADDLP Q0 Q0 32 *)
+  0x4e3d1ce2;       (* arm_AND_VEC Q2 Q7 Q29 128 *)
+  0x2ea58202;       (* arm_UMLAL_VEC Q2 Q16 Q5 32 *)
+  0x4f605415;       (* arm_SHL_VEC Q21 Q0 32 64 128 *)
+  0x6f6014e1;       (* arm_USRA_VEC Q1 Q7 32 64 128 *)
+  0x2ea58095;       (* arm_UMLAL_VEC Q21 Q4 Q5 32 *)
+  0x6f601441;       (* arm_USRA_VEC Q1 Q2 32 64 128 *)
+  0x4e083eae;       (* arm_UMOV X14 Q21 0 8 *)
+  0x4e183eaf;       (* arm_UMOV X15 Q21 1 8 *)
+  0x9b087ccc;       (* arm_MUL X12 X6 X8 *)
+  0xab0c0294;       (* arm_ADDS X20 X20 X12 *)
+  0x9bc87ccc;       (* arm_UMULH X12 X6 X8 *)
+  0x9b097ccd;       (* arm_MUL X13 X6 X9 *)
+  0xba0d02b5;       (* arm_ADCS X21 X21 X13 *)
+  0x9bc97ccd;       (* arm_UMULH X13 X6 X9 *)
+  0xba0e02d6;       (* arm_ADCS X22 X22 X14 *)
+  0xba0f02f7;       (* arm_ADCS X23 X23 X15 *)
+  0x4e083c2e;       (* arm_UMOV X14 Q1 0 8 *)
+  0x4e183c2f;       (* arm_UMOV X15 Q1 1 8 *)
+  0x9a1f03f8;       (* arm_ADC X24 XZR XZR *)
+  0xab0c02b5;       (* arm_ADDS X21 X21 X12 *)
+  0x9b037ea7;       (* arm_MUL X7 X21 X3 *)
+  0xba0d02d6;       (* arm_ADCS X22 X22 X13 *)
+  0xba0e02f7;       (* arm_ADCS X23 X23 X14 *)
+  0x9a0f0318;       (* arm_ADC X24 X24 X15 *)
+  0xa9011c26;       (* arm_STP X6 X7 X1 (Immediate_Offset (iword (&16))) *)
+  0x9b087cec;       (* arm_MUL X12 X7 X8 *)
+  0x9b097ced;       (* arm_MUL X13 X7 X9 *)
+  0x9b0a7cee;       (* arm_MUL X14 X7 X10 *)
+  0x9b0b7cef;       (* arm_MUL X15 X7 X11 *)
+  0xab0c02b5;       (* arm_ADDS X21 X21 X12 *)
+  0x9bc87cec;       (* arm_UMULH X12 X7 X8 *)
+  0xba0d02d6;       (* arm_ADCS X22 X22 X13 *)
+  0x9bc97ced;       (* arm_UMULH X13 X7 X9 *)
+  0xba0e02f7;       (* arm_ADCS X23 X23 X14 *)
+  0x9bca7cee;       (* arm_UMULH X14 X7 X10 *)
+  0xba0f0318;       (* arm_ADCS X24 X24 X15 *)
+  0x9bcb7cef;       (* arm_UMULH X15 X7 X11 *)
+  0x9a1f03f9;       (* arm_ADC X25 XZR XZR *)
+  0xab0c02cc;       (* arm_ADDS X12 X22 X12 *)
+  0xba0d02ed;       (* arm_ADCS X13 X23 X13 *)
+  0xba0e030e;       (* arm_ADCS X14 X24 X14 *)
+  0x9a0f032f;       (* arm_ADC X15 X25 X15 *)
+  0xd345fc1b;       (* arm_LSR X27 X0 5 *)
+  0x3dc00034;       (* arm_LDR Q20 X1 (Immediate_Offset (word 0)) *)
+  0x3dc00435;       (* arm_LDR Q21 X1 (Immediate_Offset (word 16)) *)
+  0xeb050090;       (* arm_SUBS X16 X4 X5 *)
+  0xda902610;       (* arm_CNEG X16 X16 Condition_CC *)
+  0xda9f23fa;       (* arm_CSETM X26 Condition_CC *)
+  0xa9026bf0;       (* arm_STP X16 X26 SP (Immediate_Offset (iword (&32))) *)
+  0xeb060090;       (* arm_SUBS X16 X4 X6 *)
+  0xda902610;       (* arm_CNEG X16 X16 Condition_CC *)
+  0xda9f23fa;       (* arm_CSETM X26 Condition_CC *)
+  0xa9036bf0;       (* arm_STP X16 X26 SP (Immediate_Offset (iword (&48))) *)
+  0xeb070090;       (* arm_SUBS X16 X4 X7 *)
+  0xda902610;       (* arm_CNEG X16 X16 Condition_CC *)
+  0xda9f23fa;       (* arm_CSETM X26 Condition_CC *)
+  0xa9046bf0;       (* arm_STP X16 X26 SP (Immediate_Offset (iword (&64))) *)
+  0xeb0600b0;       (* arm_SUBS X16 X5 X6 *)
+  0xda902610;       (* arm_CNEG X16 X16 Condition_CC *)
+  0xda9f23fa;       (* arm_CSETM X26 Condition_CC *)
+  0xa9056bf0;       (* arm_STP X16 X26 SP (Immediate_Offset (iword (&80))) *)
+  0xeb0700b0;       (* arm_SUBS X16 X5 X7 *)
+  0xda902610;       (* arm_CNEG X16 X16 Condition_CC *)
+  0xda9f23fa;       (* arm_CSETM X26 Condition_CC *)
+  0xa9066bf0;       (* arm_STP X16 X26 SP (Immediate_Offset (iword (&96))) *)
+  0xeb0700d0;       (* arm_SUBS X16 X6 X7 *)
+  0xda902610;       (* arm_CNEG X16 X16 Condition_CC *)
+  0xda9f23fa;       (* arm_CSETM X26 Condition_CC *)
+  0xa9076bf0;       (* arm_STP X16 X26 SP (Immediate_Offset (iword (&112))) *)
+  0x4e945a9e;       (* arm_UZP2 Q30 Q20 Q20 32 *)
+  0x0ea12a9c;       (* arm_XTN Q28 Q20 32 *)
+  0x4ea00a91;       (* arm_REV64_VEC Q17 Q20 32 *)
+  0x4e955ab2;       (* arm_UZP2 Q18 Q21 Q21 32 *)
+  0x0ea12ab3;       (* arm_XTN Q19 Q21 32 *)
+  0x4ea00ab4;       (* arm_REV64_VEC Q20 Q21 32 *)
   0x3cc20c4e;       (* arm_LDR Q14 X2 (Preimmediate_Offset (iword (&32))) *)
   0x3dc00459;       (* arm_LDR Q25 X2 (Immediate_Offset (word 16)) *)
   0x0ea129d5;       (* arm_XTN Q21 Q14 32 *)
@@ -189,24 +358,207 @@ let maddloop_step2_full_ops:int list = [
   0x9a0c01ef;       (* arm_ADC X15 X15 X12 *)
   0xaa0403ec;       (* arm_MOV X12 X4 *)
   0xd100077b;       (* arm_SUB X27 X27 (rvalue (word 1)) *)
-  0xb5ffed5b        (* arm_CBNZ X27 (word 2096552) *)
+  0xb5ffed5b;       (* arm_CBNZ X27 (word 2096552) *)
+  0xa9424c31;       (* arm_LDP X17 X19 X1 (Immediate_Offset (iword (&32))) *)
+  0xa9435434;       (* arm_LDP X20 X21 X1 (Immediate_Offset (iword (&48))) *)
+  0xa9417ffa;       (* arm_LDP X26 XZR SP (Immediate_Offset (iword (&16))) *)
+  0xab1c039f;       (* arm_CMN X28 X28 *)
+  0xba0c0231;       (* arm_ADCS X17 X17 X12 *)
+  0xba0d0273;       (* arm_ADCS X19 X19 X13 *)
+  0xba0e0294;       (* arm_ADCS X20 X20 X14 *)
+  0xba0f02b5;       (* arm_ADCS X21 X21 X15 *)
+  0xda9f33fc;       (* arm_CSETM X28 Condition_CS *)
+  0xa9024c31;       (* arm_STP X17 X19 X1 (Immediate_Offset (iword (&32))) *)
+  0xa9035434;       (* arm_STP X20 X21 X1 (Immediate_Offset (iword (&48))) *)
+  0xcb000021;       (* arm_SUB X1 X1 X0 *)
+  0xcb000042;       (* arm_SUB X2 X2 X0 *)
+  0x91008021;       (* arm_ADD X1 X1 (rvalue (word 32)) *)
+  0xf100075a;       (* arm_SUBS X26 X26 (rvalue (word 1)) *)
+  0xa9017ffa;       (* arm_STP X26 XZR SP (Immediate_Offset (iword (&16))) *)
+  0xf94007fe        (* arm_LDR X30 SP (Immediate_Offset (word 8)) *)
 ];;
 
-let maddloop_step2_full_mc =
-  let charlist = List.concat_map
-    (fun op32 ->
-      [Char.chr (Int.logand op32 255);
-       Char.chr (Int.logand (Int.shift_right op32 8) 255);
-       Char.chr (Int.logand (Int.shift_right op32 16) 255);
-       Char.chr (Int.logand (Int.shift_right op32 24) 255)])
-    maddloop_step2_full_ops in
-  let byte_list = Bytes.init (List.length charlist) (fun i -> List.nth charlist i) in
-  define_word_list "maddloop_step2_full_mc" (term_of_bytes byte_list);;
+let outerloop_step2_mc = define_mc_from_intlist "outerloop_step2_mc" outerloop_step2_ops;;
 
-let MADDLOOP_STEP2_FULL_EXEC = ARM_MK_EXEC_RULE maddloop_step2_full_mc;;
+let OUTERLOOP_STEP2_EXEC = ARM_MK_EXEC_RULE outerloop_step2_mc;;
+
+let outerloop_step2_labels = [
+  ("maddloop_neon", (0x29c, new_definition `outerloop_step2_label_maddloop_neon = 0x29c`));
+  (* maddloop_rotated is a virtually existing label *)
+  ("maddloop_rotated", (0x34c, new_definition `outerloop_step2_label_maddloop_rotated = 0x34c`));
+  ("inner_loop_postamble", (0x4f8, new_definition `outerloop_step2_label_inner_loop_postamble = 0x4f8`)); 
+];;
 
 
-let maddloop_step3_full_ops = [
+let outerloop_step3_ops = [
+  0xf94003e3;       (* arm_LDR X3 SP (Immediate_Offset (word 0)) *)
+  0xa9404c31;       (* arm_LDP X17 X19 X1 (Immediate_Offset (iword (&0))) *)
+  0xa9415434;       (* arm_LDP X20 X21 X1 (Immediate_Offset (iword (&16))) *)
+  0xa9402448;       (* arm_LDP X8 X9 X2 (Immediate_Offset (iword (&0))) *)
+  0xa9412c4a;       (* arm_LDP X10 X11 X2 (Immediate_Offset (iword (&16))) *)
+  0x3dc00455;       (* arm_LDR Q21 X2 (Immediate_Offset (word 16)) *)
+  0x9b037e24;       (* arm_MUL X4 X17 X3 *)
+  0x4e080c80;       (* arm_DUP_GEN Q0 X4 *)
+  0x4e955aa3;       (* arm_UZP2 Q3 Q21 Q21 32 *)
+  0x0ea12804;       (* arm_XTN Q4 Q0 32 *)
+  0x0ea12aa5;       (* arm_XTN Q5 Q21 32 *)
+  0x4ea00abc;       (* arm_REV64_VEC Q28 Q21 32 *)
+  0x2ea5c086;       (* arm_UMULL_VEC Q6 Q4 Q5 32 *)
+  0x2ea3c087;       (* arm_UMULL_VEC Q7 Q4 Q3 32 *)
+  0x4e805810;       (* arm_UZP2 Q16 Q0 Q0 32 *)
+  0x4ea09f80;       (* arm_MUL_VEC Q0 Q28 Q0 32 128 *)
+  0x6f6014c7;       (* arm_USRA_VEC Q7 Q6 32 64 128 *)
+  0x2ea3c201;       (* arm_UMULL_VEC Q1 Q16 Q3 32 *)
+  0x6ea02800;       (* arm_UADDLP Q0 Q0 32 *)
+  0x4e3d1ce2;       (* arm_AND_VEC Q2 Q7 Q29 128 *)
+  0x2ea58202;       (* arm_UMLAL_VEC Q2 Q16 Q5 32 *)
+  0x4f605400;       (* arm_SHL_VEC Q0 Q0 32 64 128 *)
+  0x6f6014e1;       (* arm_USRA_VEC Q1 Q7 32 64 128 *)
+  0x2ea58080;       (* arm_UMLAL_VEC Q0 Q4 Q5 32 *)
+  0x6f601441;       (* arm_USRA_VEC Q1 Q2 32 64 128 *)
+  0x4e083c0e;       (* arm_UMOV X14 Q0 0 8 *)
+  0x4e183c0f;       (* arm_UMOV X15 Q0 1 8 *)
+  0x9b087c8c;       (* arm_MUL X12 X4 X8 *)
+  0xab0c0231;       (* arm_ADDS X17 X17 X12 *)
+  0x9bc87c8c;       (* arm_UMULH X12 X4 X8 *)
+  0x9b097c8d;       (* arm_MUL X13 X4 X9 *)
+  0xba0d0273;       (* arm_ADCS X19 X19 X13 *)
+  0x9bc97c8d;       (* arm_UMULH X13 X4 X9 *)
+  0xba0e0294;       (* arm_ADCS X20 X20 X14 *)
+  0xba0f02b5;       (* arm_ADCS X21 X21 X15 *)
+  0x4e083c2e;       (* arm_UMOV X14 Q1 0 8 *)
+  0x4e183c2f;       (* arm_UMOV X15 Q1 1 8 *)
+  0x9a1f03f6;       (* arm_ADC X22 XZR XZR *)
+  0xab0c0273;       (* arm_ADDS X19 X19 X12 *)
+  0xba0d0294;       (* arm_ADCS X20 X20 X13 *)
+  0xba0e02b5;       (* arm_ADCS X21 X21 X14 *)
+  0x9a0f02d6;       (* arm_ADC X22 X22 X15 *)
+  0x9b037e65;       (* arm_MUL X5 X19 X3 *)
+  0x4e080ca0;       (* arm_DUP_GEN Q0 X5 *)
+  0x4e955aa3;       (* arm_UZP2 Q3 Q21 Q21 32 *)
+  0x0ea12804;       (* arm_XTN Q4 Q0 32 *)
+  0x0ea12aa5;       (* arm_XTN Q5 Q21 32 *)
+  0x4ea00abc;       (* arm_REV64_VEC Q28 Q21 32 *)
+  0x2ea5c086;       (* arm_UMULL_VEC Q6 Q4 Q5 32 *)
+  0x2ea3c087;       (* arm_UMULL_VEC Q7 Q4 Q3 32 *)
+  0x4e805810;       (* arm_UZP2 Q16 Q0 Q0 32 *)
+  0x4ea09f80;       (* arm_MUL_VEC Q0 Q28 Q0 32 128 *)
+  0x6f6014c7;       (* arm_USRA_VEC Q7 Q6 32 64 128 *)
+  0x2ea3c201;       (* arm_UMULL_VEC Q1 Q16 Q3 32 *)
+  0x6ea02800;       (* arm_UADDLP Q0 Q0 32 *)
+  0x4e3d1ce2;       (* arm_AND_VEC Q2 Q7 Q29 128 *)
+  0x2ea58202;       (* arm_UMLAL_VEC Q2 Q16 Q5 32 *)
+  0x4f605400;       (* arm_SHL_VEC Q0 Q0 32 64 128 *)
+  0x6f6014e1;       (* arm_USRA_VEC Q1 Q7 32 64 128 *)
+  0x2ea58080;       (* arm_UMLAL_VEC Q0 Q4 Q5 32 *)
+  0x6f601441;       (* arm_USRA_VEC Q1 Q2 32 64 128 *)
+  0x4e083c0e;       (* arm_UMOV X14 Q0 0 8 *)
+  0x4e183c0f;       (* arm_UMOV X15 Q0 1 8 *)
+  0x9b087cac;       (* arm_MUL X12 X5 X8 *)
+  0xab0c0273;       (* arm_ADDS X19 X19 X12 *)
+  0x9bc87cac;       (* arm_UMULH X12 X5 X8 *)
+  0x9b097cad;       (* arm_MUL X13 X5 X9 *)
+  0xba0d0294;       (* arm_ADCS X20 X20 X13 *)
+  0x9bc97cad;       (* arm_UMULH X13 X5 X9 *)
+  0xba0e02b5;       (* arm_ADCS X21 X21 X14 *)
+  0xba0f02d6;       (* arm_ADCS X22 X22 X15 *)
+  0x4e083c2e;       (* arm_UMOV X14 Q1 0 8 *)
+  0x4e183c2f;       (* arm_UMOV X15 Q1 1 8 *)
+  0x9a1f03f7;       (* arm_ADC X23 XZR XZR *)
+  0xab0c0294;       (* arm_ADDS X20 X20 X12 *)
+  0xba0d02b5;       (* arm_ADCS X21 X21 X13 *)
+  0xba0e02d6;       (* arm_ADCS X22 X22 X14 *)
+  0x9a0f02f7;       (* arm_ADC X23 X23 X15 *)
+  0xa9001424;       (* arm_STP X4 X5 X1 (Immediate_Offset (iword (&0))) *)
+  0x9b037e86;       (* arm_MUL X6 X20 X3 *)
+  0x4e080cc0;       (* arm_DUP_GEN Q0 X6 *)
+  0x4e955aa3;       (* arm_UZP2 Q3 Q21 Q21 32 *)
+  0x0ea12804;       (* arm_XTN Q4 Q0 32 *)
+  0x0ea12aa5;       (* arm_XTN Q5 Q21 32 *)
+  0x4ea00abc;       (* arm_REV64_VEC Q28 Q21 32 *)
+  0x2ea5c086;       (* arm_UMULL_VEC Q6 Q4 Q5 32 *)
+  0x2ea3c087;       (* arm_UMULL_VEC Q7 Q4 Q3 32 *)
+  0x4e805810;       (* arm_UZP2 Q16 Q0 Q0 32 *)
+  0x4ea09f80;       (* arm_MUL_VEC Q0 Q28 Q0 32 128 *)
+  0x6f6014c7;       (* arm_USRA_VEC Q7 Q6 32 64 128 *)
+  0x2ea3c201;       (* arm_UMULL_VEC Q1 Q16 Q3 32 *)
+  0x6ea02800;       (* arm_UADDLP Q0 Q0 32 *)
+  0x4e3d1ce2;       (* arm_AND_VEC Q2 Q7 Q29 128 *)
+  0x2ea58202;       (* arm_UMLAL_VEC Q2 Q16 Q5 32 *)
+  0x4f605415;       (* arm_SHL_VEC Q21 Q0 32 64 128 *)
+  0x6f6014e1;       (* arm_USRA_VEC Q1 Q7 32 64 128 *)
+  0x2ea58095;       (* arm_UMLAL_VEC Q21 Q4 Q5 32 *)
+  0x6f601441;       (* arm_USRA_VEC Q1 Q2 32 64 128 *)
+  0x4e083eae;       (* arm_UMOV X14 Q21 0 8 *)
+  0x4e183eaf;       (* arm_UMOV X15 Q21 1 8 *)
+  0x9b087ccc;       (* arm_MUL X12 X6 X8 *)
+  0xab0c0294;       (* arm_ADDS X20 X20 X12 *)
+  0x9bc87ccc;       (* arm_UMULH X12 X6 X8 *)
+  0x9b097ccd;       (* arm_MUL X13 X6 X9 *)
+  0xba0d02b5;       (* arm_ADCS X21 X21 X13 *)
+  0x9bc97ccd;       (* arm_UMULH X13 X6 X9 *)
+  0xba0e02d6;       (* arm_ADCS X22 X22 X14 *)
+  0xba0f02f7;       (* arm_ADCS X23 X23 X15 *)
+  0x4e083c2e;       (* arm_UMOV X14 Q1 0 8 *)
+  0x4e183c2f;       (* arm_UMOV X15 Q1 1 8 *)
+  0x9a1f03f8;       (* arm_ADC X24 XZR XZR *)
+  0xab0c02b5;       (* arm_ADDS X21 X21 X12 *)
+  0x9b037ea7;       (* arm_MUL X7 X21 X3 *)
+  0xba0d02d6;       (* arm_ADCS X22 X22 X13 *)
+  0xba0e02f7;       (* arm_ADCS X23 X23 X14 *)
+  0x9a0f0318;       (* arm_ADC X24 X24 X15 *)
+  0xa9011c26;       (* arm_STP X6 X7 X1 (Immediate_Offset (iword (&16))) *)
+  0x9b087cec;       (* arm_MUL X12 X7 X8 *)
+  0x9b097ced;       (* arm_MUL X13 X7 X9 *)
+  0x9b0a7cee;       (* arm_MUL X14 X7 X10 *)
+  0x9b0b7cef;       (* arm_MUL X15 X7 X11 *)
+  0xab0c02b5;       (* arm_ADDS X21 X21 X12 *)
+  0x9bc87cec;       (* arm_UMULH X12 X7 X8 *)
+  0xba0d02d6;       (* arm_ADCS X22 X22 X13 *)
+  0x9bc97ced;       (* arm_UMULH X13 X7 X9 *)
+  0xba0e02f7;       (* arm_ADCS X23 X23 X14 *)
+  0x9bca7cee;       (* arm_UMULH X14 X7 X10 *)
+  0xba0f0318;       (* arm_ADCS X24 X24 X15 *)
+  0x9bcb7cef;       (* arm_UMULH X15 X7 X11 *)
+  0x9a1f03f9;       (* arm_ADC X25 XZR XZR *)
+  0xab0c02cc;       (* arm_ADDS X12 X22 X12 *)
+  0xba0d02ed;       (* arm_ADCS X13 X23 X13 *)
+  0xba0e030e;       (* arm_ADCS X14 X24 X14 *)
+  0x9a0f032f;       (* arm_ADC X15 X25 X15 *)
+  0xd345fc1b;       (* arm_LSR X27 X0 5 *)
+  0xd100077b;       (* arm_SUB X27 X27 (rvalue (word 1)) *)
+  0x3dc00034;       (* arm_LDR Q20 X1 (Immediate_Offset (word 0)) *)
+  0x3dc00435;       (* arm_LDR Q21 X1 (Immediate_Offset (word 16)) *)
+  0xeb050090;       (* arm_SUBS X16 X4 X5 *)
+  0xda902610;       (* arm_CNEG X16 X16 Condition_CC *)
+  0xda9f23fa;       (* arm_CSETM X26 Condition_CC *)
+  0xa9026bf0;       (* arm_STP X16 X26 SP (Immediate_Offset (iword (&32))) *)
+  0xeb060090;       (* arm_SUBS X16 X4 X6 *)
+  0xda902610;       (* arm_CNEG X16 X16 Condition_CC *)
+  0xda9f23fa;       (* arm_CSETM X26 Condition_CC *)
+  0xa9036bf0;       (* arm_STP X16 X26 SP (Immediate_Offset (iword (&48))) *)
+  0xeb070090;       (* arm_SUBS X16 X4 X7 *)
+  0xda902610;       (* arm_CNEG X16 X16 Condition_CC *)
+  0xda9f23fa;       (* arm_CSETM X26 Condition_CC *)
+  0xa9046bf0;       (* arm_STP X16 X26 SP (Immediate_Offset (iword (&64))) *)
+  0xeb0600b0;       (* arm_SUBS X16 X5 X6 *)
+  0xda902610;       (* arm_CNEG X16 X16 Condition_CC *)
+  0xda9f23fa;       (* arm_CSETM X26 Condition_CC *)
+  0xa9056bf0;       (* arm_STP X16 X26 SP (Immediate_Offset (iword (&80))) *)
+  0xeb0700b0;       (* arm_SUBS X16 X5 X7 *)
+  0xda902610;       (* arm_CNEG X16 X16 Condition_CC *)
+  0xda9f23fa;       (* arm_CSETM X26 Condition_CC *)
+  0xa9066bf0;       (* arm_STP X16 X26 SP (Immediate_Offset (iword (&96))) *)
+  0xeb0700d0;       (* arm_SUBS X16 X6 X7 *)
+  0xda902610;       (* arm_CNEG X16 X16 Condition_CC *)
+  0xda9f23fa;       (* arm_CSETM X26 Condition_CC *)
+  0xa9076bf0;       (* arm_STP X16 X26 SP (Immediate_Offset (iword (&112))) *)
+  0x4e945a9e;       (* arm_UZP2 Q30 Q20 Q20 32 *)
+  0x0ea12a9c;       (* arm_XTN Q28 Q20 32 *)
+  0x4ea00a91;       (* arm_REV64_VEC Q17 Q20 32 *)
+  0x4e955ab2;       (* arm_UZP2 Q18 Q21 Q21 32 *)
+  0x0ea12ab3;       (* arm_XTN Q19 Q21 32 *)
+  0x4ea00ab4;       (* arm_REV64_VEC Q20 Q21 32 *)
   0x3cc20c4e;       (* arm_LDR Q14 X2 (Preimmediate_Offset (iword (&32))) *)
   0x3dc00459;       (* arm_LDR Q25 X2 (Immediate_Offset (word 16)) *)
   0x0ea129d5;       (* arm_XTN Q21 Q14 32 *)
@@ -506,26 +858,38 @@ let maddloop_step3_full_ops = [
   0xba0c026d;       (* arm_ADCS X13 X19 X12 *)
   0xba0c01ce;       (* arm_ADCS X14 X14 X12 *)
   0x9a0c01ef;       (* arm_ADC X15 X15 X12 *)
-  0xaa0403ec        (* arm_MOV X12 X4 *)
+  0xaa0403ec;       (* arm_MOV X12 X4 *)
+  0xa9424c31;       (* arm_LDP X17 X19 X1 (Immediate_Offset (iword (&32))) *)
+  0xa9435434;       (* arm_LDP X20 X21 X1 (Immediate_Offset (iword (&48))) *)
+  0xa9417ffa;       (* arm_LDP X26 XZR SP (Immediate_Offset (iword (&16))) *)
+  0xab1c039f;       (* arm_CMN X28 X28 *)
+  0xba0c0231;       (* arm_ADCS X17 X17 X12 *)
+  0xba0d0273;       (* arm_ADCS X19 X19 X13 *)
+  0xba0e0294;       (* arm_ADCS X20 X20 X14 *)
+  0xba0f02b5;       (* arm_ADCS X21 X21 X15 *)
+  0xda9f33fc;       (* arm_CSETM X28 Condition_CS *)
+  0xa9024c31;       (* arm_STP X17 X19 X1 (Immediate_Offset (iword (&32))) *)
+  0xa9035434;       (* arm_STP X20 X21 X1 (Immediate_Offset (iword (&48))) *)
+  0xcb000021;       (* arm_SUB X1 X1 X0 *)
+  0xcb000042;       (* arm_SUB X2 X2 X0 *)
+  0x91008021;       (* arm_ADD X1 X1 (rvalue (word 32)) *)
+  0xf100075a;       (* arm_SUBS X26 X26 (rvalue (word 1)) *)
+  0xa9017ffa;       (* arm_STP X26 XZR SP (Immediate_Offset (iword (&16))) *)
+  0xf94007fe        (* arm_LDR X30 SP (Immediate_Offset (word 8)) *)
 ];;
 
 
-let maddloop_step3_full_mc =
-  let charlist = List.concat_map
-    (fun op32 ->
-      [Char.chr (Int.logand op32 255);
-       Char.chr (Int.logand (Int.shift_right op32 8) 255);
-       Char.chr (Int.logand (Int.shift_right op32 16) 255);
-       Char.chr (Int.logand (Int.shift_right op32 24) 255)])
-    maddloop_step3_full_ops in
-  let byte_list = Bytes.init (List.length charlist) (fun i -> List.nth charlist i) in
-  define_word_list "maddloop_step3_full_mc" (term_of_bytes byte_list);;
+let outerloop_step3_mc = define_mc_from_intlist "outerloop_step3_mc" outerloop_step3_ops;;
 
-let MADDLOOP_STEP3_FULL_EXEC = ARM_MK_EXEC_RULE maddloop_step3_full_mc;;
+let OUTERLOOP_STEP3_EXEC = ARM_MK_EXEC_RULE outerloop_step3_mc;;
 
-let maddloop_step3_full_labels = [
-  new_definition `maddloop_step3_label_maddloop_neon = 0xb0`;
-  new_definition `maddloop_step3_label_innerloop_postamble = 0x30c`;  
+let outerloop_step3_labels = [
+  ("maddloop_prologue", (0x2a0, new_definition `outerloop_step3_label_maddloop_prologue = 0x2a0`));
+  ("maddloop_neon", (0x350, new_definition `outerloop_step3_label_maddloop_neon = 0x350`));
+  ("inner_loop_postamble", (0x5ac, new_definition `outerloop_step3_label_inner_loop_postamble = 0x5ac`));
+  (* inner_loop_postamble_noepilogue is a virtually existing label *)
+  ("inner_loop_postamble_noepilogue",
+    (0x750, new_definition `outerloop_step3_label_inner_loop_postamble_noepilogue = 0x750`))
 ];;
 
 
@@ -534,14 +898,16 @@ let maddloop_step3_full_labels = [
 (* ------------------------------------------------------------------------- *)
 
 (* ------------------------------------------------------------------------- *)
-(* Equivalence between the loop body, but after (k/4) - 2 iterations!        *)
+(* Equivalence between the maddloop bodies, but after (k/4) - 2 iterations!  *)
 (* maddloop_step2 will start in the middle of the loop body and stop there   *)
 (* after the iterations. maddloop_step3 will start from the maddloop_neon    *)
 (* label.                                                                    *)
 (* ------------------------------------------------------------------------- *)
 
 let step2_body_in_regs, step2_body_out_regs =
-    approximate_input_output_regs (snd MADDLOOP_STEP3_FULL_EXEC) [(0xb0,0x308)];;
+    approximate_input_output_regs (snd OUTERLOOP_STEP3_EXEC)
+      [(fst (assoc "maddloop_neon" outerloop_step3_labels),
+        fst (assoc "inner_loop_postamble" outerloop_step3_labels) - 4)];;
 let step2_body_in_xregs = filter (fun t -> type_of t = `:(armstate,int64)component`)
     step2_body_in_regs;;
 let step2_body_in_qregs = filter (fun t -> type_of t = `:(armstate,int128)component`)
@@ -571,6 +937,8 @@ let step2_body_eq_mems = new_definition
     (exists a. bignum_from_memory (m_precalc,12*(k DIV 4 - 1)) s1 = a /\
                 bignum_from_memory (m_precalc,12*(k DIV 4 - 1)) s1' = a)`;;
 
+let step2_body_eq_unfold_rules = [step2_body_eq_mems;step2_body_eq_xregs;step2_body_eq_qregs;
+        mk_equiv_regs];;
 
 let step2_body_eqin = new_definition
   `forall s1 s1' z m m_precalc sp k.
@@ -621,22 +989,26 @@ let step2_body_maychanges =
 
 let equiv_goal1 = mk_equiv_statement
     `ALL (nonoverlapping (z,8 * k))
-     [word pc:int64,LENGTH maddloop_step2_full_mc; word pc2:int64,LENGTH maddloop_step3_full_mc;
+     [word pc:int64,LENGTH outerloop_step2_mc; word pc2:int64,LENGTH outerloop_step3_mc;
       sp:int64,128; m:int64,8*k; m_precalc:int64,8*12*(k DIV 4 - 1)] /\
      aligned 16 (sp:int64) /\ 8 divides k /\ 12 <= k /\ k < 2 EXP 61`
     step2_body_eqin
     step2_body_eqout
-    maddloop_step2_full_mc 0xb0 0xb0
+    outerloop_step2_mc
+    (fst (assoc "maddloop_rotated" outerloop_step2_labels))
+    (fst (assoc "maddloop_rotated" outerloop_step2_labels))
     step2_body_maychanges
-    maddloop_step3_full_mc 0xb0 0x30c
+    outerloop_step3_mc
+    (fst (assoc "maddloop_neon" outerloop_step3_labels))
+    (fst (assoc "inner_loop_postamble" outerloop_step3_labels))
     step2_body_maychanges
     `\(s:armstate). 151 * (k DIV 4 - 2)` `\(s:armstate). 151 * (k DIV 4 - 2)`;;
 
 
-let MADDLOOP_STEP2_STEP3_EQUIV = prove(equiv_goal1,
+let OUTERLOOP_MADDLOOP_STEP2_STEP3_EQUIV = prove(equiv_goal1,
   REWRITE_TAC[MODIFIABLE_SIMD_REGS;SOME_FLAGS;
     ALLPAIRS;ALL;NONOVERLAPPING_CLAUSES;
-    fst MADDLOOP_STEP2_FULL_EXEC; fst MADDLOOP_STEP3_FULL_EXEC] THEN
+    fst OUTERLOOP_STEP2_EXEC; fst OUTERLOOP_STEP3_EXEC] THEN
   REPEAT STRIP_TAC THEN
 
   ABBREV_TAC `k4 = k DIV 4` THEN
@@ -651,7 +1023,11 @@ let MADDLOOP_STEP2_STEP3_EQUIV = prove(equiv_goal1,
   SUBGOAL_THEN `3 <= k4` ASSUME_TAC THENL [ ASM_ARITH_TAC; ALL_TAC ] THEN
 
   (* iterates 'k / 4 - 2' times, where k is the number of words in modulus *)
-  ENSURES2_WHILE_PAUP_TAC `1` `k4 - 1:num` `pc+0xb0` `pc+0xb0` `pc2+0xb0` `pc2+0x308`
+  ENSURES2_WHILE_PAUP_TAC `1` `k4 - 1:num`
+    `pc+outerloop_step2_label_maddloop_rotated`
+    `pc+outerloop_step2_label_maddloop_rotated`
+    `pc2+outerloop_step3_label_maddloop_neon`
+    `pc2+(outerloop_step3_label_inner_loop_postamble-4)`
     `\(i:num) s1 s1'.
       // loop counter
       read X27 s1 = word (k4 - i) /\
@@ -673,7 +1049,12 @@ let MADDLOOP_STEP2_STEP3_EQUIV = prove(equiv_goal1,
     `\(i:num). 150`
     (* pre steps *)`0` `0`
     (* post steps *)`0` `1`
-    (* num backedges *)`0` `1` THEN REPEAT CONJ_TAC THENL [
+    (* num backedges *)`0` `1`
+  THEN SUBST1_TAC
+    ((REWRITE_CONV (map (snd o snd) (outerloop_step2_labels @ outerloop_step3_labels))
+      THENC NUM_REDUCE_CONV) `outerloop_step3_label_inner_loop_postamble-4`)
+  THEN REWRITE_TAC (map (snd o snd) (outerloop_step2_labels @ outerloop_step3_labels))
+  THEN REPEAT CONJ_TAC THENL [
       (* loop count which is k4-1 > 0. *)
       FIRST_ASSUM (fun th -> MP_TAC (MATCH_MP DIVIDES_LE th)) THEN ASM_ARITH_TAC;
 
@@ -697,12 +1078,10 @@ let MADDLOOP_STEP2_STEP3_EQUIV = prove(equiv_goal1,
       REPEAT STRIP_TAC THEN
       ENSURES2_INIT_TAC "s0" "s0'" THEN
       UNDISCH_THEN `k DIV 4 = k4` (fun th -> SUBST_ALL_TAC th THEN ASSUME_TAC th) THEN
-      RULE_ASSUM_TAC(REWRITE_RULE[
-        step2_body_eq_mems;step2_body_eq_xregs;step2_body_eq_qregs;
-        mk_equiv_regs;BIGNUM_FROM_MEMORY_BYTES]) THEN
+      RULE_ASSUM_TAC(REWRITE_RULE (step2_body_eq_unfold_rules @ [BIGNUM_FROM_MEMORY_BYTES])) THEN
       REPEAT SPLIT_FIRST_CONJ_ASSUM_TAC THEN
       DESTRUCT_EXISTS_ASSUMS_TAC THEN
-      ARM_STUTTER_RIGHT_TAC MADDLOOP_STEP3_FULL_EXEC [1] "'" None THEN
+      ARM_STUTTER_RIGHT_TAC OUTERLOOP_STEP3_EXEC [1] "'" None THEN
       REPEAT_N 2 ENSURES_FINAL_STATE'_TAC THEN
       SUBGOAL_THEN `~(val (word (k4 - (i + 1)):int64) = 0)` MP_TAC THENL [
         IMP_REWRITE_TAC[VAL_WORD_EQ;DIMINDEX_64] THEN ASM_ARITH_TAC;
@@ -714,8 +1093,7 @@ let MADDLOOP_STEP2_STEP3_EQUIV = prove(equiv_goal1,
           [FIRST_X_ASSUM MATCH_ACCEPT_TAC ORELSE ASM_MESON_TAC[BIGNUM_FROM_MEMORY_BYTES];
           ALL_TAC]) THEN
         REPEAT CONJ_TAC THENL (replicate
-          (REWRITE_TAC[step2_body_eq_mems;step2_body_eq_xregs;step2_body_eq_qregs;
-                       BIGNUM_FROM_MEMORY_BYTES;mk_equiv_regs] THEN
+          (REWRITE_TAC(step2_body_eq_unfold_rules @ [BIGNUM_FROM_MEMORY_BYTES]) THEN
            ASM_REWRITE_TAC[] THEN ASM_MESON_TAC[])
           3);
 
@@ -730,12 +1108,10 @@ let MADDLOOP_STEP2_STEP3_EQUIV = prove(equiv_goal1,
       (* postcond! *)
       REWRITE_TAC[step2_body_eqout;SUB_REFL;MULT_0] THEN
       ENSURES2_INIT_TAC "s0" "s0'" THEN
-      RULE_ASSUM_TAC(REWRITE_RULE[
-        step2_body_eq_mems;step2_body_eq_xregs;step2_body_eq_qregs;
-        mk_equiv_regs;BIGNUM_FROM_MEMORY_BYTES]) THEN
+      RULE_ASSUM_TAC(REWRITE_RULE (step2_body_eq_unfold_rules @ [BIGNUM_FROM_MEMORY_BYTES])) THEN
       REPEAT SPLIT_FIRST_CONJ_ASSUM_TAC THEN
       DESTRUCT_EXISTS_ASSUMS_TAC THEN
-      ARM_STUTTER_RIGHT_TAC MADDLOOP_STEP3_FULL_EXEC [1] "'" None THEN
+      ARM_STUTTER_RIGHT_TAC OUTERLOOP_STEP3_EXEC [1] "'" None THEN
       REPEAT_N 2 ENSURES_FINAL_STATE'_TAC THEN
       CONJ_TAC THENL [
         SUBGOAL_THEN `(val (word (k4 - (k4 - 1 + 1)):int64) = 0)`
@@ -749,8 +1125,7 @@ let MADDLOOP_STEP2_STEP3_EQUIV = prove(equiv_goal1,
         [ ASM_ARITH_TAC; ALL_TAC ] THEN
         ASM_REWRITE_TAC[] THEN
         REPEAT CONJ_TAC THENL (replicate
-          (REWRITE_TAC[step2_body_eq_mems;step2_body_eq_xregs;step2_body_eq_qregs;
-                      BIGNUM_FROM_MEMORY_BYTES;mk_equiv_regs] THEN
+          (REWRITE_TAC (step2_body_eq_unfold_rules @ [BIGNUM_FROM_MEMORY_BYTES]) THEN
            ASM_MESON_TAC[]) 3);
 
         CONJ_TAC THENL [
@@ -822,8 +1197,7 @@ let MADDLOOP_STEP2_STEP3_EQUIV = prove(equiv_goal1,
       ALL_TAC
     ] THEN
 
-    REWRITE_TAC[BIGNUM_FROM_MEMORY_BYTES;
-      step2_body_eq_mems;step2_body_eq_xregs;step2_body_eq_qregs;mk_equiv_regs] THEN
+    REWRITE_TAC(BIGNUM_FROM_MEMORY_BYTES::step2_body_eq_unfold_rules) THEN
     DISCH_THEN (LABEL_TAC "HSPLITTER") (* the 3 part splitter *) THEN
     SUBGOAL_THEN `(i' + 1) + 1 = i' + 2` SUBST_ALL_TAC THENL [ARITH_TAC;ALL_TAC] THEN
 
@@ -851,20 +1225,20 @@ let MADDLOOP_STEP2_STEP3_EQUIV = prove(equiv_goal1,
     ABBREV_TAC `mi' = word_add m (word (8 * 4 * i')):int64` THEN
     ABBREV_TAC `m_precalci' = word_add m_precalc (word (8 * 12 * i')):int64` THEN
     SUBGOAL_THEN `ALL (nonoverlapping (word_add zi' (word 32):int64,64))
-        [(word pc2:int64, LENGTH maddloop_step3_full_mc);(word pc, LENGTH maddloop_step2_full_mc);
+        [(word pc2:int64, LENGTH outerloop_step3_mc);(word pc, LENGTH outerloop_step2_mc);
          (sp:int64,128); (m:int64,8*4*k4); (m_precalc:int64,8*12*(k4 - 1));
          (word_add mi' (word 32):int64,64); (m_precalci':int64,128);
          (z:int64,8*4*(i'+1))]`
         MP_TAC THENL [
       MAP_EVERY EXPAND_TAC ["zi'";"mi'";"m_precalci'"] THEN
 
-      REWRITE_TAC[ALL; NONOVERLAPPING_CLAUSES;fst MADDLOOP_STEP2_FULL_EXEC;
-                  fst MADDLOOP_STEP3_FULL_EXEC] THEN
+      REWRITE_TAC[ALL; NONOVERLAPPING_CLAUSES;fst OUTERLOOP_STEP2_EXEC;
+                  fst OUTERLOOP_STEP3_EXEC] THEN
       REPEAT (CONJ_TAC THENL [NONOVERLAPPING_TAC; ALL_TAC]) THEN NONOVERLAPPING_TAC;
 
       DISCH_THEN (fun th -> MP_TAC (
-        REWRITE_RULE[ALL; NONOVERLAPPING_CLAUSES;fst MADDLOOP_STEP2_FULL_EXEC;
-                    fst MADDLOOP_STEP3_FULL_EXEC] th)) THEN
+        REWRITE_RULE[ALL; NONOVERLAPPING_CLAUSES;fst OUTERLOOP_STEP2_EXEC;
+                    fst OUTERLOOP_STEP3_EXEC] th)) THEN
       STRIP_TAC
     ] THEN
 
@@ -1013,9 +1387,9 @@ let MADDLOOP_STEP2_STEP3_EQUIV = prove(equiv_goal1,
     FIND_ABBREV_THEN "zi'" (fun th ->
       UNDISCH_THEN (concl th) (LABEL_TAC "DO_NOT_CLEAR")) THEN
 
-    EQUIV_STEPS_TAC [("equal",0,105,0,105)] MADDLOOP_STEP2_FULL_EXEC MADDLOOP_STEP3_FULL_EXEC THEN
+    EQUIV_STEPS_TAC [("equal",0,105,0,105)] OUTERLOOP_STEP2_EXEC OUTERLOOP_STEP3_EXEC THEN
     (* backedge! *)
-    ARM_STUTTER_LEFT_TAC MADDLOOP_STEP2_FULL_EXEC [106;107] None THEN
+    ARM_STUTTER_LEFT_TAC OUTERLOOP_STEP2_EXEC [106;107] None THEN
     SUBGOAL_THEN `~(val (word_sub (word (k4 - (i' + 1))) (word 1):int64) = 0)` MP_TAC THENL [
       REWRITE_TAC[VAL_EQ_0] THEN
       IMP_REWRITE_TAC[WORD_SUB2] THEN
@@ -1034,8 +1408,8 @@ let MADDLOOP_STEP2_STEP3_EQUIV = prove(equiv_goal1,
       ("replace",147,148,145,146);
       ("equal",148,150,146,148);
       ("replace",150,151,148,149);
-      ("equal",151,152,149,150)] MADDLOOP_STEP2_FULL_EXEC MADDLOOP_STEP3_FULL_EXEC THEN
-    ARM_STUTTER_RIGHT_TAC MADDLOOP_STEP3_FULL_EXEC [151] "'" None THEN
+      ("equal",151,152,149,150)] OUTERLOOP_STEP2_EXEC OUTERLOOP_STEP3_EXEC THEN
+    ARM_STUTTER_RIGHT_TAC OUTERLOOP_STEP3_EXEC [151] "'" None THEN
 
     REPEAT_N 2 ENSURES_FINAL_STATE'_TAC THEN
     (* Prove remaining clauses from the postcondition *)
@@ -1082,7 +1456,9 @@ let MADDLOOP_STEP2_STEP3_EQUIV = prove(equiv_goal1,
 (* Building input state equiv. *)
 
 let step2_prolog_in_regs, step2_prolog_out_regs = approximate_input_output_regs
-    (snd MADDLOOP_STEP3_FULL_EXEC) [(0x00,0xac)];;
+    (snd OUTERLOOP_STEP3_EXEC)
+    [(fst (assoc "maddloop_prologue" outerloop_step3_labels),
+      fst (assoc "maddloop_neon" outerloop_step3_labels) - 4)];;
 let step2_prolog_in_regs = union step2_prolog_in_regs
     (subtract step2_body_in_regs step2_prolog_out_regs);;
 let step2_prolog_out_regs = union step2_prolog_out_regs step2_body_in_regs;;
@@ -1179,32 +1555,38 @@ let step2_prolog_eqout = new_definition
     step2_prolog_eqout_xregs(s1,s1') /\
     step2_prolog_eqout_qregs(s1,s1'))`;;
 
+let step2_prolog_eq_unfold_rules = [
+    step2_prolog_eqin_xregs;step2_prolog_eqin_qregs;step2_prolog_eq_mems;
+    step2_prolog_eqout_xregs;step2_prolog_eqout_qregs;mk_equiv_regs];;
+
 
 let equiv_goal2 = mk_equiv_statement
     `ALL (nonoverlapping (z,8 * k))
-     [word pc:int64,LENGTH maddloop_step2_full_mc; word pc2:int64,LENGTH maddloop_step3_full_mc;
+     [word pc:int64,LENGTH outerloop_step2_mc; word pc2:int64,LENGTH outerloop_step3_mc;
       sp:int64,128; m:int64,8*k; m_precalc:int64,8*12*(k DIV 4 - 1)] /\
      aligned 16 (sp:int64) /\ 8 divides k /\ 12 <= k /\ k < 2 EXP 61`
     step2_prolog_eqin
     step2_prolog_eqout
-    maddloop_step2_full_mc 0x0 0xb0
+    outerloop_step2_mc
+    (fst (assoc "maddloop_neon" outerloop_step2_labels))
+    (fst (assoc "maddloop_rotated" outerloop_step2_labels))
     step2_prolog_maychanges
-    maddloop_step3_full_mc 0x0 0xb0
+    outerloop_step3_mc
+    (fst (assoc "maddloop_prologue" outerloop_step3_labels))
+    (fst (assoc "maddloop_neon" outerloop_step3_labels))
     step2_prolog_maychanges
     `\(s:armstate). 44` `\(s:armstate). 44`;;
 
 
-let MADDLOOP_STEP2_STEP3_PROLOG_EQUIV = prove(equiv_goal2,
+let OUTERLOOP_PROLOG_STEP2_STEP3_EQUIV = prove(equiv_goal2,
   REWRITE_TAC[MODIFIABLE_SIMD_REGS;SOME_FLAGS;
     ALLPAIRS;ALL;NONOVERLAPPING_CLAUSES;
-    fst MADDLOOP_STEP2_FULL_EXEC; fst MADDLOOP_STEP3_FULL_EXEC] THEN
+    fst OUTERLOOP_STEP2_EXEC; fst OUTERLOOP_STEP3_EXEC] THEN
   REPEAT STRIP_TAC THEN
 
   (** Initialize **)
   EQUIV_INITIATE_TAC step2_prolog_eqin THEN
-  RULE_ASSUM_TAC(REWRITE_RULE[
-    step2_prolog_eq_mems;step2_prolog_eqin_qregs;step2_prolog_eqin_xregs;
-    mk_equiv_regs; BIGNUM_FROM_MEMORY_BYTES]) THEN
+  RULE_ASSUM_TAC(REWRITE_RULE (step2_prolog_eq_unfold_rules @ [BIGNUM_FROM_MEMORY_BYTES])) THEN
   REPEAT SPLIT_FIRST_CONJ_ASSUM_TAC THEN
   DESTRUCT_EXISTS_ASSUMS_TAC THEN
 
@@ -1232,7 +1614,7 @@ let MADDLOOP_STEP2_STEP3_PROLOG_EQUIV = prove(equiv_goal2,
     MAP_EVERY (fun state_term ->
       MP_TAC (GSYM (SPECL [`4*k4:num`;`m:int64`;state_term;`4 + j`]
           BIGDIGIT_BIGNUM_FROM_MEMORY)) THEN
-      COND_CASES_TAC THENL [ALL_TAC; ASM_ARITH_TAC] THEN
+      COND_CASES_TAC THENL [ALL_TAC; SIMPLE_ARITH_TAC] THEN
       DISCH_THEN (fun th ->
         MP_TAC (REWRITE_RULE[VAL_WORD_GALOIS; DIMINDEX_64; BIGDIGIT_BOUND; LEFT_ADD_DISTRIB] th)) THEN
       DISCH_THEN SUBST1_TAC) [`s0:armstate`;`s0':armstate`] THEN
@@ -1258,7 +1640,7 @@ let MADDLOOP_STEP2_STEP3_PROLOG_EQUIV = prove(equiv_goal2,
     MAP_EVERY (fun state_term ->
       MP_TAC (GSYM (SPECL [`12:num`;`word_add sp (word 32):int64`;state_term;`j:num`]
           BIGDIGIT_BIGNUM_FROM_MEMORY)) THEN
-      COND_CASES_TAC THENL [ALL_TAC; ASM_ARITH_TAC] THEN
+      COND_CASES_TAC THENL [ALL_TAC; SIMPLE_ARITH_TAC] THEN
       DISCH_THEN (fun th ->
         MP_TAC (REWRITE_RULE[VAL_WORD_GALOIS; DIMINDEX_64; BIGDIGIT_BOUND;
             WORD_ADD_ASSOC_CONSTS; LEFT_ADD_DISTRIB] th)) THEN
@@ -1283,7 +1665,7 @@ let MADDLOOP_STEP2_STEP3_PROLOG_EQUIV = prove(equiv_goal2,
     MAP_EVERY (fun state_term ->
       MP_TAC (GSYM (SPECL [`12 * (k4 - 1):num`;`m_precalc:int64`;state_term;`j:num`]
           BIGDIGIT_BIGNUM_FROM_MEMORY)) THEN
-      COND_CASES_TAC THENL [ALL_TAC; ASM_ARITH_TAC] THEN
+      COND_CASES_TAC THENL [ALL_TAC; SIMPLE_ARITH_TAC] THEN
       DISCH_THEN (fun th ->
         MP_TAC (REWRITE_RULE[VAL_WORD_GALOIS; DIMINDEX_64; BIGDIGIT_BOUND; LEFT_ADD_DISTRIB] th)) THEN
       DISCH_THEN SUBST1_TAC) [`s0:armstate`;`s0':armstate`] THEN
@@ -1308,7 +1690,7 @@ let MADDLOOP_STEP2_STEP3_PROLOG_EQUIV = prove(equiv_goal2,
     MAP_EVERY (fun state_term ->
       MP_TAC (GSYM (SPECL [`4 * k4`;`z:int64`;state_term;`4 + j:num`]
           BIGDIGIT_BIGNUM_FROM_MEMORY)) THEN
-      COND_CASES_TAC THENL [ALL_TAC; ASM_ARITH_TAC] THEN
+      COND_CASES_TAC THENL [ALL_TAC; SIMPLE_ARITH_TAC] THEN
       DISCH_THEN (fun th ->
         MP_TAC (REWRITE_RULE[VAL_WORD_GALOIS; DIMINDEX_64; BIGDIGIT_BOUND;
                 LEFT_ADD_DISTRIB;ARITH_RULE`8*4=32`] th)) THEN
@@ -1327,16 +1709,14 @@ let MADDLOOP_STEP2_STEP3_PROLOG_EQUIV = prove(equiv_goal2,
   EQUIV_STEPS_TAC [
       ("replace",0,1,0,1);("equal",1,39,1,39);("replace",39,40,39,40);
       ("replace",40,44,40,44)]
-    MADDLOOP_STEP2_FULL_EXEC MADDLOOP_STEP3_FULL_EXEC THEN
+    OUTERLOOP_STEP2_EXEC OUTERLOOP_STEP3_EXEC THEN
 
   REPEAT_N 2 ENSURES_FINAL_STATE'_TAC THEN
   (* Prove remaining clauses from the postcondition *)
   ASM_REWRITE_TAC[] THEN
   REPEAT CONJ_TAC THENL [
     (** SUBGOAL 1. Outputs **)
-    ASM_REWRITE_TAC[step2_prolog_eqout;
-                step2_prolog_eq_mems;step2_prolog_eqout_xregs;step2_prolog_eqout_qregs;
-                mk_equiv_regs;BIGNUM_FROM_MEMORY_BYTES] THEN
+    ASM_REWRITE_TAC(step2_prolog_eqout::BIGNUM_FROM_MEMORY_BYTES::step2_prolog_eq_unfold_rules) THEN
     FIND_ABBREV_THEN "k" (SUBST_ALL_TAC o GSYM) THEN
     ASM_REWRITE_TAC[ARITH_RULE`(4 * x) DIV 4 = x`; MESON[]`!(x:A). exists y. x = y`] THEN
     NO_TAC;
@@ -1358,19 +1738,21 @@ let MADDLOOP_STEP2_STEP3_PROLOG_EQUIV = prove(equiv_goal2,
 (* input states *)
 
 let step2_epilog_in_regs, step2_epilog_out_regs = approximate_input_output_regs
-    (snd MADDLOOP_STEP3_FULL_EXEC) [(0x30c,0x4ac)];;
+    (snd OUTERLOOP_STEP3_EXEC)
+    [(fst (assoc "inner_loop_postamble" outerloop_step3_labels),
+      fst (assoc "inner_loop_postamble_noepilogue" outerloop_step3_labels) - 4)];;
 
 let step2_epilog_in_xregs = filter (fun t -> type_of t = `:(armstate,int64)component`)
     step2_epilog_in_regs;;
 let step2_epilog_in_qregs = filter (fun t -> type_of t = `:(armstate,int128)component`)
     step2_epilog_in_regs;;
 
+(* exclude pointers and loop counter because they will explicitly appear in step2_epilog_eqin *)
+let step2_epilog_in_xregs = subtract step2_epilog_in_xregs [`X27`;`X1`;`X2`;`SP`;`X30`];;
+
 (* Loop body's output regs equivalence must cover epilogue's input regs equiv. *)
 assert (subset step2_epilog_in_xregs step2_body_out_xregs);;
 assert (subset step2_epilog_in_qregs step2_body_out_qregs);;
-
-(* exclude pointers and loop counter because they will explicitly appear in step2_epilog_eqin *)
-let step2_epilog_in_xregs = subtract step2_epilog_in_xregs [`X27`;`X1`;`X2`;`SP`;`X30`];;
 
 let step2_epilog_eqin_xregs = new_definition
   (mk_eq
@@ -1465,25 +1847,394 @@ let step2_epilog_eqout = new_definition
     step2_epilog_eqout_qregs(s1,s1'))`;;
 
 
+let step2_epilog_eq_unfold_rules = [
+  step2_epilog_eqin_xregs; step2_epilog_eqin_qregs; step2_epilog_eq_mems;
+  step2_epilog_eqout_xregs; step2_epilog_eqout_qregs; mk_equiv_regs
+];;
+
+
 let equiv_goal3 = mk_equiv_statement
     `ALL (nonoverlapping (z,8 * k))
-     [word pc:int64,LENGTH maddloop_step2_full_mc; word pc2:int64,LENGTH maddloop_step3_full_mc;
+     [word pc:int64,LENGTH outerloop_step2_mc; word pc2:int64,LENGTH outerloop_step3_mc;
       sp:int64,128; m:int64,8*k; m_precalc:int64,8*12*(k DIV 4 - 1)] /\
      aligned 16 (sp:int64) /\ 8 divides k /\ 12 <= k /\ k < 2 EXP 61`
     step2_epilog_eqin
     step2_epilog_eqout
-    maddloop_step2_full_mc 0xb0 0x25c
+    outerloop_step2_mc
+    (fst (assoc "maddloop_rotated" outerloop_step2_labels))
+    (fst (assoc "inner_loop_postamble" outerloop_step2_labels))
     step2_epilog_maychanges_left
-    maddloop_step3_full_mc 0x30c 0x4b0
+    outerloop_step3_mc
+    (fst (assoc "inner_loop_postamble" outerloop_step3_labels))
+    (fst (assoc "inner_loop_postamble_noepilogue" outerloop_step3_labels))
     step2_epilog_maychanges_right
     `\(s:armstate). 107` `\(s:armstate). 105`;;
 
 
-let MADDLOOP_STEP2_STEP3_EPILOG_EQUIV = prove(equiv_goal3,
+let OUTERLOOP_EPILOG_STEP2_STEP3_EQUIV = prove(equiv_goal3,
   REWRITE_TAC[MODIFIABLE_SIMD_REGS;SOME_FLAGS;
     ALLPAIRS;ALL;NONOVERLAPPING_CLAUSES;
-    fst MADDLOOP_STEP2_FULL_EXEC; fst MADDLOOP_STEP3_FULL_EXEC] THEN
+    fst OUTERLOOP_STEP2_EXEC; fst OUTERLOOP_STEP3_EXEC] THEN
   REPEAT STRIP_TAC THEN
+
+  (* prepare memory loads *)
+  ABBREV_TAC `k4 = k DIV 4` THEN
+  SUBGOAL_THEN `3 <= k4 /\ k4 < 2 EXP 59` MP_TAC THENL [ASM_ARITH_TAC;STRIP_TAC]
+  THEN
+  SUBGOAL_THEN `k = 4 * k4` (LABEL_TAC "HK_DO_NOT_CLEAR") THENL [
+    UNDISCH_TAC `8 divides k` THEN
+    REWRITE_TAC[DIVIDES_DIV_MULT;ARITH_RULE`k DIV 8 = k DIV (4*2)`;GSYM DIV_DIV] THEN
+    ASM_ARITH_TAC;
+    ALL_TAC
+  ] THEN
+
+  (* split 'bignum_from_memory (z,k) s = bignum_from_memory (z,k) s2' into two parts:
+      1. bignum_from_memory (z,k-1) s = ..
+      2. bignum_from_memory (z+4*(k-1),4) s = .. *)
+  SUBGOAL_THEN `!(s:armstate) (s2:armstate).
+      (exists a. bignum_from_memory (z:int64,4*k4) s = a /\ bignum_from_memory (z,4*k4) s2 = a)
+      <=>
+      ((exists a1. bignum_from_memory (z,(4*k4-4)) s = a1 /\ bignum_from_memory (z,(4*k4-4)) s2 = a1) /\
+       (exists a2. bignum_from_memory (word_add z (word (8*(4*k4-4))),4) s = a2 /\
+                   bignum_from_memory (word_add z (word (8*(4*k4-4))),4) s2 = a2))`
+      (LABEL_TAC "Hmemsplit") THENL [
+    REPEAT STRIP_TAC THEN EQ_TAC THENL [
+      STRIP_TAC THEN REPEAT CONJ_TAC THENL [
+        SUBGOAL_THEN `MIN (4*k4) (4 * k4-4) = 4 * k4-4` ASSUME_TAC
+        THENL [ ASM_ARITH_TAC; ALL_TAC] THEN
+        ASM_MESON_TAC[LOWDIGITS_BIGNUM_FROM_MEMORY];
+
+        SUBGOAL_THEN `4 = 4*k4 - (4*k4-4)` (LABEL_TAC "H") THENL [ ASM_ARITH_TAC; ALL_TAC ] THEN
+        ASM_MESON_TAC[HIGHDIGITS_BIGNUM_FROM_MEMORY]
+      ];
+
+      REPEAT STRIP_TAC THEN
+      SUBGOAL_THEN `4 * k4 = (4 * k4 - 4) + 4` SUBST1_TAC THENL [ ASM_ARITH_TAC; ALL_TAC ] THEN
+      ASM_MESON_TAC[BIGNUM_FROM_MEMORY_SPLIT]
+    ];
+
+    ALL_TAC
+  ] THEN
+
+  (** Initialize **)
+  EQUIV_INITIATE_TAC step2_epilog_eqin THEN
+  REMOVE_THEN "HK_DO_NOT_CLEAR" (fun th -> SUBST_ALL_TAC th THEN LABEL_TAC "HK_DO_NOT_CLEAR" th) THEN
+  RULE_ASSUM_TAC(REWRITE_RULE(step2_epilog_eq_unfold_rules @
+      [BIGNUM_FROM_MEMORY_BYTES; ARITH_RULE`(4 * x) DIV 4 = x`])) THEN
+  REMOVE_THEN "Hmemsplit" (fun th -> RULE_ASSUM_TAC(REWRITE_RULE[th]) THEN LABEL_TAC "Hmemsplit" th) THEN
+  REPEAT SPLIT_FIRST_CONJ_ASSUM_TAC THEN
+  DESTRUCT_EXISTS_ASSUMS_TAC THEN
+
+  (* define m_precalc' to avoid negative offsets appearing in equations. *)
+
+  ABBREV_TAC `m_precalc' = word_add m_precalc (word (8 * 12 * (k4 - 2))):int64` THEN
+  SUBGOAL_THEN `word_sub m_precalc' (word (8 * 12 * (k4 - 2))) = m_precalc:int64` ASSUME_TAC THENL
+  [ EXPAND_TAC "m_precalc'" THEN CONV_TAC WORD_RULE; ALL_TAC ] THEN
+  REPEAT (FIRST_X_ASSUM (fun th -> let c = concl th in
+    if can (find_term (fun t -> t = `X30`)) c then
+      (FIND_ABBREV_THEN "m_precalc" (fun ath -> MP_TAC (REWRITE_RULE[GSYM ath] th)))
+    else NO_TAC)) THEN
+  REWRITE_TAC[WORD_RULE
+    `word_add (word_sub x (word y)) (word z):int64 = word_add x (word_sub (word z) (word y))`] THEN
+  SUBGOAL_THEN `word_sub (word (8 * 12 * (k4 - 1))) (word (8 * 12 * (k4 - 2))):int64 =
+                word 96` (LABEL_TAC "Hm_precalc'") THENL [
+    IMP_REWRITE_TAC[WORD_SUB2] THEN CONJ_TAC THENL [
+      AP_TERM_TAC THEN ASM_ARITH_TAC;
+      ASM_ARITH_TAC
+    ];
+    ALL_TAC
+  ] THEN
+  REMOVE_THEN "Hm_precalc'" (fun th -> SUBST_ALL_TAC th THEN LABEL_TAC "Hm_precalc'" th) THEN
+  REPEAT STRIP_TAC THEN
+  SUBGOAL_THEN `nonoverlapping_modulo (2 EXP 64) (val (z:int64),8 * 4 * k4)
+      (val (m_precalc':int64),96)` ASSUME_TAC THENL [
+
+    EXPAND_TAC "m_precalc'" THEN NONOVERLAPPING_TAC;
+    ALL_TAC
+  ] THEN
+
+  (* load from sp.. *)
+  SUBGOAL_THEN
+    `forall j. j < 8 ==> exists a1.
+        read (memory :> bytes64 (word_add sp (word (64 + 8 * j)))) s0 = a1 /\
+        read (memory :> bytes64 (word_add sp (word (64 + 8 * j)))) s0' = a1`
+  MP_TAC THENL [
+    REPEAT STRIP_TAC THEN REWRITE_TAC[WORD_ADD_ASSOC_CONSTS;LEFT_ADD_DISTRIB] THEN
+
+    MAP_EVERY (fun state_term ->
+      MP_TAC (GSYM (SPECL [`12:num`;`word_add sp (word 32):int64`;state_term;`4 + j:num`]
+          BIGDIGIT_BIGNUM_FROM_MEMORY)) THEN
+      COND_CASES_TAC THENL [ALL_TAC; SIMPLE_ARITH_TAC] THEN
+      DISCH_THEN (fun th ->
+        MP_TAC (REWRITE_RULE[VAL_WORD_GALOIS; DIMINDEX_64; BIGDIGIT_BOUND;
+            WORD_ADD_ASSOC_CONSTS; LEFT_ADD_DISTRIB; ADD_ASSOC] th)) THEN
+      CONV_TAC (ONCE_DEPTH_CONV NUM_REDUCE_CONV) THEN
+      DISCH_THEN SUBST1_TAC) [`s0:armstate`;`s0':armstate`] THEN
+
+    ASM_MESON_TAC[BIGNUM_FROM_MEMORY_BYTES];
+
+    ALL_TAC
+  ] THEN
+  CONV_TAC (LAND_CONV (EXPAND_CASES_CONV THENC REWRITE_CONV[LEFT_ADD_DISTRIB] THENC
+                       ONCE_DEPTH_CONV NUM_REDUCE_CONV)) THEN
+  STRIP_TAC THEN
+
+  (* load from m_precalc (x30).. *)
+  SUBGOAL_THEN
+    `forall j. j < 12 ==> exists a2.
+        read (memory :> bytes64 (word_add m_precalc' (word (8 * j)))) s0 = a2 /\
+        read (memory :> bytes64 (word_add m_precalc' (word (8 * j)))) s0' = a2`
+  MP_TAC THENL [
+    REPEAT STRIP_TAC THEN
+    EXPAND_TAC "m_precalc'" THEN
+    REWRITE_TAC[WORD_ADD_ASSOC_CONSTS] THEN
+
+    MAP_EVERY (fun state_term ->
+      MP_TAC (GSYM (SPECL [`12 * (k4 - 1):num`;`m_precalc:int64`;
+                           state_term;`(12 * (k4 - 2) + j)`]
+          BIGDIGIT_BIGNUM_FROM_MEMORY)) THEN
+      COND_CASES_TAC THENL [ALL_TAC; SIMPLE_ARITH_TAC] THEN
+      DISCH_THEN (fun th ->
+        MP_TAC (REWRITE_RULE[VAL_WORD_GALOIS; DIMINDEX_64; BIGDIGIT_BOUND;
+                             WORD_ADD_ASSOC_CONSTS; LEFT_ADD_DISTRIB] th)) THEN
+      DISCH_THEN SUBST1_TAC) [`s0:armstate`;`s0':armstate`] THEN
+
+    ASM_MESON_TAC[BIGNUM_FROM_MEMORY_BYTES];
+
+    ALL_TAC
+  ] THEN
+  CONV_TAC (LAND_CONV (EXPAND_CASES_CONV THENC REWRITE_CONV[LEFT_ADD_DISTRIB] THENC
+                       ONCE_DEPTH_CONV NUM_REDUCE_CONV)) THEN
+  STRIP_TAC THEN
+
+  (* load from z (x1).. *)
+  SUBGOAL_THEN
+    `forall j. j < 2 ==> exists a3.
+        read (memory :> bytes64 (word_add z (word (8 * ((4 * k4 - 4) + 2 + j))))) s0 = a3 /\
+        read (memory :> bytes64 (word_add z (word (8 * ((4 * k4 - 4) + 2 + j))))) s0' = a3`
+  MP_TAC THENL [
+    REPEAT STRIP_TAC THEN REWRITE_TAC[WORD_ADD_ASSOC_CONSTS;LEFT_ADD_DISTRIB] THEN
+
+    MAP_EVERY (fun state_term ->
+      MP_TAC (GSYM (SPECL [`4`;`word_add z (word (8 * (4 * k4 - 4))):int64`;state_term;`2 + j:num`]
+          BIGDIGIT_BIGNUM_FROM_MEMORY)) THEN
+      COND_CASES_TAC THENL [ALL_TAC; SIMPLE_ARITH_TAC] THEN
+      DISCH_THEN (fun th ->
+        MP_TAC (REWRITE_RULE[VAL_WORD_GALOIS; DIMINDEX_64; BIGDIGIT_BOUND; WORD_ADD_ASSOC_CONSTS;
+                LEFT_ADD_DISTRIB] th)) THEN
+      DISCH_THEN SUBST1_TAC) [`s0:armstate`;`s0':armstate`] THEN
+
+    ASM_MESON_TAC[BIGNUM_FROM_MEMORY_BYTES];
+
+    ALL_TAC
+  ] THEN
+  CONV_TAC (LAND_CONV
+    (EXPAND_CASES_CONV THENC REWRITE_CONV[LEFT_ADD_DISTRIB] THENC
+     ONCE_DEPTH_CONV NUM_REDUCE_CONV THENC REWRITE_CONV[WORD_ADD_0])) THEN
+  STRIP_TAC THEN
+
+  (* start *)
+  REMOVE_ABBREV_THEN "m_precalc" (LABEL_TAC "m_precalc_DO_NOT_CLEAR") THEN
+  REMOVE_ABBREV_THEN "m_precalc'" (K ALL_TAC) THEN
+
+  EQUIV_STEPS_TAC [
+      ("equal",0,105,0,105);
+      ("delete",105,107,105,105) (* exit the branch of the maddloop (step2) *)]
+    OUTERLOOP_STEP2_EXEC OUTERLOOP_STEP3_EXEC THEN
+
+  REPEAT_N 2 ENSURES_FINAL_STATE'_TAC THEN
+  (* Prove remaining clauses from the postcondition *)
+  ASM_REWRITE_TAC[] THEN
+  REPEAT CONJ_TAC THENL [
+    (** SUBGOAL 1. Outputs **)
+    ASM_REWRITE_TAC(step2_epilog_eqout::BIGNUM_FROM_MEMORY_BYTES::step2_epilog_eq_unfold_rules) THEN
+    ASM_REWRITE_TAC[ARITH_RULE`(4 * x) DIV 4 = x`; MESON[] `!(x:A). exists y. x = y`] THEN
+    EXPAND_TAC "m_precalc" THEN ASM_REWRITE_TAC[WORD_ADD_SUB] THEN
+    (* only one goal here.. let's expand memory :> bytes. *)
+    REWRITE_TAC[GSYM BIGNUM_FROM_MEMORY_BYTES] THEN
+    REPEAT (ONCE_REWRITE_TAC[BIGNUM_FROM_MEMORY_EXPAND] THEN
+            CHANGED_TAC (CONV_TAC (ONCE_DEPTH_CONV NUM_REDUCE_CONV))) THEN
+    REWRITE_TAC[WORD_ADD_ASSOC_CONSTS] THEN CONV_TAC (ONCE_DEPTH_CONV NUM_REDUCE_CONV) THEN
+    ASM_REWRITE_TAC[] THEN MESON_TAC[];
+
+    (** SUBGOAL 2. Maychange left **)
+    DISCARD_ASSUMPTIONS_TAC (fun th -> free_in `s0':armstate` (concl th)) THEN
+    MONOTONE_MAYCHANGE_TAC;
+
+    (** SUBGOAL 3. Maychange right **)
+    DISCARD_ASSUMPTIONS_TAC (fun th -> free_in `s0:armstate` (concl th)) THEN
+    MONOTONE_MAYCHANGE_TAC
+  ]);;
+
+
+let STEP2_PROLOG_EQOUT_IMPLIES_BODY_EQIN =
+  prove(`forall s1 s1' z m m_precalc sp k.
+    step2_prolog_eqout (s1,s1') z m m_precalc sp k ==>
+    step2_body_eqin (s1,s1') z m m_precalc sp k`,
+    REWRITE_TAC([step2_prolog_eqout;step2_body_eqin] @
+        step2_prolog_eq_unfold_rules @ step2_body_eq_unfold_rules) THEN
+    REPEAT GEN_TAC THEN STRIP_TAC THEN ASM_REWRITE_TAC[]
+    THEN MESON_TAC[]);;
+
+let STEP2_BODY_EQOUT_IMPLIES_EPILOGUE_EQIN =
+  prove(`forall s1 s1' z m m_precalc sp k.
+    step2_body_eqout (s1,s1') z m m_precalc sp k ==>
+    step2_epilog_eqin (s1,s1') z m m_precalc sp k`,
+    REWRITE_TAC([step2_body_eqout;step2_epilog_eqin] @
+        step2_body_eq_unfold_rules @ step2_epilog_eq_unfold_rules) THEN
+    REPEAT GEN_TAC THEN STRIP_TAC THEN ASM_REWRITE_TAC[]
+    THEN MESON_TAC[]);;
+
+
+let OUTERLOOP_PROLOG_MADDLOOP_EPILOG_STEP2_STEP3_FULL_EQUIV =
+  let prolog_body_equiv = prove_equiv_seq_composition
+    OUTERLOOP_PROLOG_STEP2_STEP3_EQUIV
+    OUTERLOOP_MADDLOOP_STEP2_STEP3_EQUIV
+    STEP2_PROLOG_EQOUT_IMPLIES_BODY_EQIN in
+  prove_equiv_seq_composition prolog_body_equiv OUTERLOOP_EPILOG_STEP2_STEP3_EQUIV
+    STEP2_BODY_EQOUT_IMPLIES_EPILOGUE_EQIN;;
+
+
+
+(* ------------------------------------------------------------------------- *)
+(* Equivalence between the outerloop blocks.                                 *)
+(* ------------------------------------------------------------------------- *)
+
+(* input states *)
+
+let step2_outerloop_in_regs, step2_outerloop_out_regs = approximate_input_output_regs
+    (snd OUTERLOOP_STEP3_EXEC)
+    [(0x0, fst (assoc "maddloop_prologue" outerloop_step3_labels) - 4)];;
+
+let step2_outerloop_in_xregs = filter (fun t -> type_of t = `:(armstate,int64)component`)
+    step2_outerloop_in_regs;;
+let step2_outerloop_in_qregs = filter (fun t -> type_of t = `:(armstate,int128)component`)
+    step2_outerloop_in_regs;;
+
+(* exclude pointers and loop counter because they will explicitly appear in step2_outerloop_eqin *)
+let step2_outerloop_in_xregs = subtract step2_outerloop_in_xregs [`X0`;`X1`;`X2`;`SP`];;
+
+let step2_outerloop_eqin_xregs = new_definition
+  (mk_eq
+    (`(step2_outerloop_eqin_xregs:armstate#armstate->bool) (s1,s1')`,
+      list_mk_icomb "mk_equiv_regs"
+      [mk_list (step2_outerloop_in_xregs,`:(armstate,int64)component`);`(s1:armstate,s1':armstate)`]));;
+let step2_outerloop_eqin_qregs = new_definition
+  (mk_eq
+    (`(step2_outerloop_eqin_qregs:armstate#armstate->bool) (s1,s1')`,
+      list_mk_icomb "mk_equiv_regs"
+      [mk_list (step2_outerloop_in_qregs,`:(armstate,int128)component`);`(s1:armstate,s1':armstate)`]));;
+let step2_outerloop_eq_mems = new_definition
+  `(step2_outerloop_eq_mems:int64->int64->int64->int64->num->armstate#armstate->bool)
+      z m sp m_precalc k (s1,s1') <=>
+    (exists a. bignum_from_memory (z,k) s1  = a /\ bignum_from_memory (z,k) s1' = a) /\
+    (exists a. bignum_from_memory (m,k) s1  = a /\ bignum_from_memory (m,k) s1' = a) /\
+    (exists a. read (memory :> bytes64 sp) s1 = a /\
+                read (memory :> bytes64 sp) s1' = a) /\
+    (exists a. bignum_from_memory (word_add sp (word 32),12) s1 = a /\
+                bignum_from_memory (word_add sp (word 32),12) s1' = a) /\
+    (exists a. bignum_from_memory (m_precalc,12*(k DIV 4 - 1)) s1 = a /\
+                bignum_from_memory (m_precalc,12*(k DIV 4 - 1)) s1' = a)`;;
+
+let step2_outerloop_eqin = new_definition
+  `forall s1 s1' z m m_precalc sp k.
+   (step2_outerloop_eqin:(armstate#armstate)->int64->int64->int64->int64->num->bool)
+        (s1,s1') z m m_precalc sp k <=>
+   (read X0 s1 = word (8 * (k - 4)) /\ read X0 s1' = word (8 * (k - 4)) /\
+    read X1 s1 = z /\ read X1 s1' = z /\
+    read X2 s1 = m /\ read X2 s1' = m /\
+    read SP s1 = sp /\ read SP s1' = sp /\
+    read X30 s1 = m_precalc /\ read X30 s1' = m_precalc /\
+    step2_outerloop_eq_mems z m sp m_precalc k (s1,s1') /\
+    step2_outerloop_eqin_xregs (s1,s1') /\
+    step2_outerloop_eqin_qregs (s1,s1'))`;;
+
+
+(* output states and maychange *)
+
+let step2_outerloop_out_xregs,step2_outerloop_out_regs2 = partition
+    (fun t -> type_of t = `:(armstate,int64)component`) step2_outerloop_out_regs;;
+let step2_outerloop_out_qregs,step2_outerloop_out_flags = partition
+    (fun t -> type_of t = `:(armstate,int128)component`) step2_outerloop_out_regs2;;
+
+(* Loop body's output regs equivalence must cover outerloop's input regs equiv. *)
+assert (subset step2_prolog_in_xregs step2_outerloop_out_xregs);;
+assert (subset step2_prolog_in_qregs (`Q29`::step2_outerloop_out_qregs));;
+
+let step2_outerloop_maychanges_left =
+  end_itlist (fun x y -> mk_icomb (mk_icomb (`,,`,x),y))
+    [mk_icomb (`MAYCHANGE`,mk_list (step2_outerloop_out_xregs, `:(armstate,int64)component`));
+     mk_icomb (`MAYCHANGE`,mk_list (step2_outerloop_out_qregs, `:(armstate,int128)component`));
+     mk_icomb (`MAYCHANGE`,mk_list (step2_outerloop_out_flags, `:(armstate,bool)component`));
+     `MAYCHANGE [memory :> bytes (z:int64,8 * k)]`;
+     `MAYCHANGE [PC]`];;
+let step2_outerloop_maychanges_right = step2_outerloop_maychanges_left;;
+
+(* exclude pointers and loop counter because they will explicitly appear in step2_epilog_eqout *)
+let step2_outerloop_maychange_xregs = subtract step2_outerloop_out_xregs [`X27`;`X1`;`X2`;`SP`;`X30`];;
+
+let step2_outerloop_eqout_xregs = new_definition
+  (mk_eq
+    (`(step2_outerloop_eqout_xregs:armstate#armstate->bool) (s1,s1')`,
+      list_mk_icomb "mk_equiv_regs"
+      [mk_list (step2_outerloop_out_xregs,`:(armstate,int64)component`);`(s1:armstate,s1':armstate)`]));;
+let step2_outerloop_eqout_qregs = new_definition
+  (mk_eq
+    (`(step2_outerloop_eqout_qregs:armstate#armstate->bool) (s1,s1')`,
+      list_mk_icomb "mk_equiv_regs"
+      [mk_list (step2_outerloop_in_qregs,`:(armstate,int128)component`);`(s1:armstate,s1':armstate)`]));;
+
+let step2_outerloop_eqout = new_definition
+  `forall s1 s1' z m m_precalc sp k.
+  (step2_outerloop_eqout:(armstate#armstate)->int64->int64->int64->int64->num->bool)
+        (s1,s1') z m m_precalc sp k <=>
+   (read X27 s1 = word (k DIV 4 - 1) /\ read X27 s1 = word (k DIV 4 - 2) /\
+    read X1 s1 = z /\ read X1 s1' = z /\
+    read X2 s1 = m /\ read X2 s1' = m /\
+    read SP s1 = sp /\ read SP s1' = sp /\
+    read X30 s1 = m_precalc /\ read X30 s1' = m_precalc /\
+    step2_outerloop_eq_mems z m sp m_precalc k (s1,s1') /\
+    step2_outerloop_eqin_xregs (s1,s1') /\
+    step2_outerloop_eqin_qregs (s1,s1'))`;;
+
+let equiv_goal4 = mk_equiv_statement
+    `ALL (nonoverlapping (z,8 * k))
+     [word pc:int64,LENGTH outerloop_step2_mc; word pc2:int64,LENGTH outerloop_step3_mc;
+      sp:int64,128; m:int64,8*k; m_precalc:int64,8*12*(k DIV 4 - 1)] /\
+     aligned 16 (sp:int64) /\ 8 divides k /\ 12 <= k /\ k < 2 EXP 61`
+    step2_outerloop_eqin
+    step2_outerloop_eqout
+    outerloop_step2_mc
+    0x0
+    (fst (assoc "maddloop_neon" outerloop_step2_labels))
+    step2_epilog_maychanges_left
+    outerloop_step3_mc
+    0x0
+    (fst (assoc "maddloop_prologue" outerloop_step3_labels))
+    step2_epilog_maychanges_right
+    `\(s:armstate). 167` `\(s:armstate). 168`;;
+
+(*
+let OUTERLOOP_OUTERLOOP_STEP2_STEP3_EQUIV = prove(equiv_goal4,
+  REWRITE_TAC[MODIFIABLE_SIMD_REGS;SOME_FLAGS;
+    ALLPAIRS;ALL;NONOVERLAPPING_CLAUSES;
+    fst OUTERLOOP_STEP2_EXEC; fst OUTERLOOP_STEP3_EXEC] THEN
+  REPEAT STRIP_TAC THEN
+
+  (** Initialize **)
+  EQUIV_INITIATE_TAC step2_outerloop_eqin THEN
+  RULE_ASSUM_TAC(REWRITE_RULE[
+    step2_outerloop_eq_mems;step2_outerloop_eqin_qregs;step2_outerloop_eqin_xregs;
+    mk_equiv_regs; BIGNUM_FROM_MEMORY_BYTES]) THEN
+  REPEAT SPLIT_FIRST_CONJ_ASSUM_TAC THEN
+  DESTRUCT_EXISTS_ASSUMS_TAC THEN
+
+  EQUIV_STEPS_TAC [
+      ("equal",0,167,0,167);
+      ("insert",167,167,167,168) (* exit the branch of the maddloop (step2) *)]
+    OUTERLOOP_STEP2_EXEC OUTERLOOP_STEP3_EXEC THEN
+
+
 
   (* prepare memory loads *)
   ABBREV_TAC `k4 = k DIV 4` THEN
@@ -1661,7 +2412,7 @@ let MADDLOOP_STEP2_STEP3_EPILOG_EQUIV = prove(equiv_goal3,
   EQUIV_STEPS_TAC [
       ("equal",0,105,0,105);
       ("delete",105,107,105,105) (* exit the branch of the maddloop (step2) *)]
-    MADDLOOP_STEP2_FULL_EXEC MADDLOOP_STEP3_FULL_EXEC THEN
+    OUTERLOOP_STEP2_EXEC OUTERLOOP_STEP3_EXEC THEN
 
   REPEAT_N 2 ENSURES_FINAL_STATE'_TAC THEN
   (* Prove remaining clauses from the postcondition *)
@@ -1688,3 +2439,5 @@ let MADDLOOP_STEP2_STEP3_EPILOG_EQUIV = prove(equiv_goal3,
     DISCARD_ASSUMPTIONS_TAC (fun th -> free_in `s0:armstate` (concl th)) THEN
     MONOTONE_MAYCHANGE_TAC
   ]);;
+
+*)
